src/ConcreteEvidence.v
@@ -15,7 +15,7 @@ Inductive EvidenceC: Set :=
 | mtc: EvidenceC
 | uuc: ASP_ID -> BS -> EvidenceC -> EvidenceC
 | ggc: BS -> EvidenceC -> EvidenceC
-| hhc: BS -> EvidenceC -> EvidenceC (* TODO: remove Ev param *)
+(*| hhc: BS -> EvidenceC -> EvidenceC *) (* TODO: remove Ev param *)
                           (*
 | nnc: N_ID -> BS -> EvidenceC -> EvidenceC
 | ssc: EvidenceC -> EvidenceC -> EvidenceC
@@ -57,9 +57,9 @@ Inductive Ev_Shape: EvidenceC -> Evidence -> Prop :=
 | ggt: forall p bs e et,
     Ev_Shape e et ->
     Ev_Shape (ggc bs e) (gg p et)
-| hht: forall p bs e et,
+(*| hht: forall p bs e et,
     Ev_Shape e et ->
-    Ev_Shape (hhc bs e) (hh p et)
+    Ev_Shape (hhc bs e) (hh p et) *)
              (*
 | nnt: forall bs e et i i',
     Ev_Shape e et ->
